ex 7.4, 7.5, 7.6

Chap7ex.thy
@@ -26,7 +26,7 @@ lemma "skip c \<Longrightarrow> c \<sim> SKIP"
   using assign_simp apply auto
    apply (metis Seq Skip)
   by (meson Skip big_step.IfFalse big_step.IfTrue)
-  
+
 lemma skip_while_aux: "\<lbrakk> (WHILE b DO c, s) \<Rightarrow> s'; bval b s \<rbrakk> \<Longrightarrow> \<not>bval b s'"
   apply (induct "WHILE b DO c" s s' rule: big_step_induct)
   by blast+
@@ -34,7 +34,7 @@ lemma skip_while_aux: "\<lbrakk> (WHILE b DO c, s) \<Rightarrow> s'; bval b s \<
 lemma skip_while: "bval b s \<Longrightarrow> \<not>(WHILE b DO c \<sim> SKIP)"
 text \<open>if the loop halts after n iterations, then @{term "(WHILE b DO c, s) \<Rightarrow> sn"} and since
 @{term "bval b s \<noteq> bval b sn"}, @{term "s \<noteq> sn"}. otherwise, the loop never halts,
-so for all t, @{term "(WHILE b DO c, s) \<Rightarrow> t"} does not hold.\<close> 
+so for all t, @{term "(WHILE b DO c, s) \<Rightarrow> t"} does not hold.\<close>
   using skip_while_aux by blast
 
 lemma "WHILE b DO c \<sim> SKIP = skip (WHILE b DO c)"
@@ -51,7 +51,7 @@ lemma
 let c2 = x ::= Plus (V x) (N 1) in
 IF (Bc True) THEN c1 ELSE c2 \<sim> SKIP"
   apply clarsimp
-  by (metis Chap7_2.IfE big_step.IfTrue bval.simps(1)) 
+  by (metis Chap7_2.IfE big_step.IfTrue bval.simps(1))
 
 lemma "c \<sim> SKIP \<Longrightarrow> skip c"
   apply (induction c)
@@ -79,7 +79,7 @@ function (sequential) deskip :: "com \<Rightarrow> com" where
 | "deskip (v ::= a) = v ::= a"
 | "deskip (SKIP;; p) = deskip p"
 | "deskip (p;; SKIP) = deskip p"
-| "deskip (p;; q) = (let (p', q') = (deskip p, deskip q) in 
+| "deskip (p;; q) = (let (p', q') = (deskip p, deskip q) in
 if (p', q') = (p, q) then p;; q else deskip (p';; q'))"
 | "deskip (IF b THEN p ELSE q) = IF b THEN deskip p ELSE deskip q"
 | "deskip (WHILE b DO p) = WHILE b DO deskip p"
@@ -134,5 +134,89 @@ lemma "deskip c \<sim> c"
                       apply (blast+)[14]
          apply ((meson Chap7_2.SeqE Seq)+)[7]
   using sim_while_cong by presburger
+
+inductive astep :: "aexp * state \<Rightarrow> aexp \<Rightarrow> bool" (infix "\<leadsto>" 50) where
+"(V x, s) \<leadsto> N (s x)"
+| "(Plus (N i) (N j), s) \<leadsto> N (i + j)"
+| "(e, s) \<leadsto> e' \<Longrightarrow> (Plus e e'', s) \<leadsto> Plus e' e''"
+| "(e, s) \<leadsto> e' \<Longrightarrow> (Plus (N i) e, s) \<leadsto> Plus (N i) e'"
+
+lemma "(a, s) \<leadsto> a' \<Longrightarrow> aval a s = aval a' s"
+  thm astep.induct astep.induct[split_format (complete)]
+proof (induction rule: astep.induct[split_format (complete)])
+  fix x s
+  show "aval (V x) s = aval (N (s x)) s" by simp
+next
+  fix i j s
+  show "aval (Plus (N i) (N j)) s = aval (N (i + j)) s" by simp
+next
+  fix e s e' e''
+  assume "(e, s) \<leadsto> e'" and "aval e s = aval e' s"
+  thus "aval (Plus e e'') s = aval (Plus e' e'') s" by simp
+next
+  fix e s e' i
+  assume "(e, s) \<leadsto> e'" and "aval e s = aval e' s"
+  thus "aval (Plus (N i) e) s = aval (Plus (N i) e') s" by simp
+qed
+
+lemma "IF And b1 b2 THEN c1 ELSE c2 \<sim> IF b1 THEN (IF b2 THEN c1 ELSE c2) ELSE c2"
+  apply clarsimp
+  subgoal for s t
+    apply (cases "bval b1 s")
+    by fastforce+
+  done
+
+lemma helper_7_5: "\<not>(WHILE Bc True DO c, s) \<Rightarrow> t"
+  apply clarsimp
+  by (induct "WHILE Bc True DO c" s t rule: big_step_induct; simp)
+
+lemma "\<not>WHILE And b1 b2 DO c \<sim> WHILE b1 DO WHILE b2 DO c"
+  if "b1 \<equiv> Eq (N 0) (V ''x'')" and "b2 \<equiv> Bc True" and "c \<equiv> ''x'' ::= Plus (V ''x'') (N 1)"
+and "s \<equiv> (\<lambda>_. 0) :: char list \<Rightarrow> int" and "t \<equiv> <''x'' := 1::int>"
+  apply clarsimp
+  apply (rule exI[where x=s])
+  apply (rule exI[where x=t])
+  apply (subgoal_tac "(WHILE And b1 b2 DO c, s) \<Rightarrow> t")
+   apply (subgoal_tac "\<not> (WHILE b1 DO WHILE b2 DO c, s) \<Rightarrow> t")
+    apply simp
+   apply (thin_tac "_")
+   apply clarsimp
+   apply (erule Chap7_2.WhileE)
+  defer
+  unfolding that apply simp
+   apply (rule WhileTrue[where t=t])
+     apply simp
+    apply (subgoal_tac "t = (\<lambda>_. 0)(''x'' := 1)")
+  apply (simp add: assign_simp)
+  unfolding that(5)
+    apply (simp add: null_state_def)
+   apply (rule WhileFalse; simp)
+  using helper_7_5 by blast
+
+abbreviation Or where "Or b1 b2 \<equiv> Not (And (Not b1) (Not b2))"
+
+lemma "WHILE Or b1 b2 DO c \<sim> WHILE Or b1 b2 DO c;; WHILE b1 DO c"
+  apply clarsimp
+  subgoal for s t
+  apply (rule iffI)
+     apply (induct "WHILE Or b1 b2 DO c" s t rule: big_step_induct; clarsimp)
+      apply (metis Seq WhileTrue bval.simps(2) bval.simps(3))
+    apply (metis Seq WhileFalse bval.simps(2) bval.simps(3))
+    by (metis Chap7_2.SeqE Chap7_2.WhileE bval.simps(2) bval.simps(3) skip_while_aux)
+  done
+
+definition DoWhile :: "com \<Rightarrow> bexp \<Rightarrow> com" ("(DO _ WHILE _)")where
+"DO c WHILE b \<equiv> c ;; WHILE b DO c"
+
+fun dewhile :: "com \<Rightarrow> com" where
+"dewhile SKIP = SKIP"
+| "dewhile (x ::= a) = x ::= a"
+| "dewhile (p ;; q) = dewhile p ;; dewhile q"
+| "dewhile (IF b THEN p ELSE q) = IF b THEN (dewhile p) ELSE (dewhile q)"
+| "dewhile (WHILE b DO c) = IF (Not b) THEN SKIP ELSE DO c WHILE b"
+
+lemma "dewhile c \<sim> c"
+  apply (induct c)
+  using DoWhile_def Seq Skip big_step.IfFalse big_step.IfTrue by auto
 
 end
